Flapjack/Stack.lean
@@ -46,6 +46,7 @@ inductive StackProg (α : Type u) where
   | skip
   | const (destination value : Nat)
   | inst (instruction : WordInst)
+  | shMem (operator : WordMemOp) (source address : Nat)
   | get (destination : Nat) (store : StackStore)
   | set (store : StackStore) (source : Nat)
   | arith (operator : BinOp) (destination left right : Nat)
